checks/SemantChecks.v
@@ -16,21 +16,31 @@ Section TypeDec_CHECKS.
   Ltac inv H := inversion H; subst; clear H.
   Ltac inv_all :=
     repeat match goal with
-    | [ H : wt_prog _ _ _ |- _ ] => inv H
-    | [ H : wt_exp _ _ _ _ _ |- _ ] => inv H
-    | [ H : wt_op _ _ _ _ |- _ ] => inv H
-    | [ H : Some _ = Some _ |- _ ] => inv H
     | [ H : Some _ = None |- _ ] => inv H
     | [ H : None = Some _ |- _ ] => inv H
-    | [ H : None = None |- _ ] => inv H
-    | [ H : Types.actual_ty _ Types.STRING = Some _ |- _] => unfold Types.actual_ty in H; simpl in H
-    | [ H : Types.actual_ty _ Types.INT = Some _ |- _] => unfold Types.actual_ty in H; simpl in H
+    | [ H : Some _ = Some _ |- _ ] => inv H
+    | [ H : wt_op _ _ _ _ |- _ ] => inv H
+    | [ H : wt_fields _ _ _ _ |- _ ] => inv H
+    | [ H : wt_ty _ _ _ _ _ |- _ ] => inv H
+    | [ H : wt_tydec_heads _ _ _ |- _ ] => inv H
+    | [ H : wt_tydecs _ _ _ _ _ |- _ ] => inv H
+    | [ H : wt_formals_heads _ _ _ |- _ ] => inv H
+    | [ H : wt_formals _ _ _ _ |- _ ] => inv H
+    | [ H : wt_fundec_heads _ _ _ |- _ ] => inv H
+    | [ H : wt_exp _ _ _ _ _ |- _ ] => inv H
+    | [ H : wt_explist _ _ _ _ _ |- _ ] => inv H
+    | [ H : wt_var _ _ _ _ _ |- _ ] => inv H
+    | [ H : wt_dec _ _ _ _ _ |- _ ] => inv H
+    | [ H : wt_declist _ _ _ _ _ |- _ ] => inv H
+    | [ H : wt_fundecs _ _ _ _ _  |- _ ] => inv H
+    | [ H : wt_prog _ _ _ |- _ ] => inv H
+    | [ H : Types.actual_ty _ _ = Some _ |- _ ] => unfold Types.actual_ty in H; simpl in H
     end; simpl in *; try discriminate.
 
   Ltac solve :=
     match goal with
     | [ |- checkEx ?E ] => unfold checkEx, E, transProg; simpl; eauto
-    | [ |- failEx ?E ] => unfold failEx, E, not; intros; inv_all
+    | [ |- failEx ?E ] => unfold failEx, E, not; intros; repeat inv_all
     end.
 
   Example ex1 : checkEx EX1.ex.
@@ -64,6 +74,33 @@ Section TypeDec_CHECKS.
   Proof. solve. Qed.
 
   Example ex11 : failEx EX11.ex.
+  Proof. solve. Qed.
+
+  Example ex12 : checkEx EX12.ex.
+  Proof. solve. Qed.
+
+  Example ex13 : failEx EX13.ex.
+  Proof. solve. Qed.
+
+  (* Very slow *)
+  Example ex14 : failEx EX14.ex.
+  Proof. solve. Qed.
+
+  Example ex15 : failEx EX15.ex.
+  Proof. solve. Qed.
+
+  Example ex16 : failEx EX16.ex.
+  Proof. solve. Qed.
+
+  Example ex17 : failEx EX17.ex.
+  Proof. solve. Qed.
+
+  (* Slow *)
+  Example ex18 : failEx EX18.ex.
+  Proof. solve. Qed.
+
+  (* Slow *)
+  Example ex19 : failEx EX19.ex.
   Proof. solve. Qed.
 
 End TypeDec_CHECKS.
